theories/glogic.v
@@ -1,5 +1,5 @@
 Require Export g_stlc.
-From stdpp Require Import sets.
+Require Import sets.
 
 
 (*************************)
@@ -20,29 +20,37 @@ Module Type SQ_SET.
     forall f s t, t ∈ sq_set_map f s <-> exists a, a ∈ s /\ t = f a.
 End SQ_SET.
 
-(*
-Notation "x :: X" := (X ∪ {[x]}) : stlc_scope.
-Notation "X :: x" := (X ∪ {[x]}) (in custom stlc_tm at level 60, left associativity) : stlc_scope.
-*)
 
 Module GLogic (SqSet : SQ_SET).
   Export SqSet.
   Export GStlcTheories.
 
-  (*
-  Record sequent : Type := sq_build {
-    sq_context : context;
-    sq_premises : sq_set;
-    sq_conclusion : tm;
-    _ : forall t, t ∈ sq_premises -> has_type sq_context t ty_prp;
-    _ : has_type sq_context sq_conclusion ty_prp
-  }.
-  *)
-
-  Definition is_form C t := has_type C t ty_prp.
-  Definition wf_sq_set C (l : sq_set) := forall t, t ∈ l -> has_type C t ty_prp.
+  Notation is_form C t := (has_type C t ty_prp).
+  Definition wf_sq_set C (l : sq_set) := forall t, t ∈ l -> is_form C t.
 
   Definition wf_sequent C (p : sq_set) c := wf_sq_set C p /\ is_form C c.
+
+  Instance wf_sequent_Proper : Proper ((=) ==> (≡) ==> (=) ==> iff) wf_sequent.
+  Proof.
+    intros C ? <- p q E c ? <-.
+    unfold wf_sequent, wf_sq_set. intuition; set_solver.
+  Qed.
+
+
+  (***********************)
+  (** ** Deduction rules *)
+  (***********************)
+
+  Notation "∅" := empty (in custom stlc_ty) : stlc_scope.
+  Notation "∅" := empty (in custom stlc_tm) : stlc_scope.
+  Notation "∅" := empty : stdpp_scope.
+  Infix "∪" := union (in custom stlc_tm at level 50) : stlc_scope.
+  Infix "∪" := union : stdpp_scope.
+  Notation "s +; x" := (s ∪ {[x]}) (in custom stlc_tm at level 50, left associativity) : stlc_scope.
+  Notation "s +; x" := (s ∪ {[x]}) (at level 50, left associativity) : stlc_scope.
+  Notation "{[ x ]}" := (singleton x) (in custom stlc_tm) : stlc_scope.
+  Notation "{[ x ]}" := (singleton x) : stdpp_scope.
+
 
   Inductive is_derivable_wf : context -> sq_set -> tm -> Prop :=
     | wrl_set C l m c :
@@ -56,11 +64,11 @@ Module GLogic (SqSet : SQ_SET).
         is_derivable_wf C {[a]} b
     | wrl_cut C l m b c :
         is_derivable_wf C l b ->
-        is_derivable_wf C (m ∪ {[b]}) c ->
+        is_derivable_wf C (m +; b) c ->
         is_derivable_wf C (l ∪ m) c
     | wrl_cL C l b c :
-        is_derivable_wf C (l ∪ {[b; b]}) c ->
-        is_derivable_wf C (l ∪ {[b]}) c
+        is_derivable_wf C (l +; b +; b) c ->
+        is_derivable_wf C (l +; b) c
     | wrl_wL C l m b :
         (forall a, a ∈ l -> has_type C a ty_prp) ->
         is_derivable_wf C m b ->
@@ -71,9 +79,9 @@ Module GLogic (SqSet : SQ_SET).
     | wrl_topR C :
         is_derivable_wf C ∅ gtm_top
     | wrl_orL C l b c d :
-        is_derivable_wf C (l ∪ {[b]}) c ->
-        is_derivable_wf C (l ∪ {[d]}) c ->
-        is_derivable_wf C (l ∪ {[ <{ b \/ d }> ]}) c
+        is_derivable_wf C (l +; b) c ->
+        is_derivable_wf C (l +; d) c ->
+        is_derivable_wf C (l +; <{ b \/ d }>) c
     | wrl_orR1 C l b c :
         has_type C c ty_prp ->
         is_derivable_wf C l b ->
@@ -84,27 +92,27 @@ Module GLogic (SqSet : SQ_SET).
         is_derivable_wf C l <{ b \/ c }>
     | wrl_andL1 C l b c d :
         has_type C d ty_prp ->
-        is_derivable_wf C (l ∪ {[b]}) c ->
-        is_derivable_wf C (l ∪ {[ <{ b /\ d }> ]}) c
+        is_derivable_wf C (l +; b) c ->
+        is_derivable_wf C (l +; <{ b /\ d }>) c
     | wrl_andL2 C l b c d :
         has_type C b ty_prp ->
-        is_derivable_wf C (l ∪ {[d]}) c ->
-        is_derivable_wf C (l ∪ {[ <{ b /\ d }> ]}) c
+        is_derivable_wf C (l +; d) c ->
+        is_derivable_wf C (l +; <{ b /\ d }>) c
     | wrl_andR C l b c :
         is_derivable_wf C l b ->
         is_derivable_wf C l c ->
         is_derivable_wf C l <{ b /\ c }>
     | wrl_impL C l b c d :
         is_derivable_wf C l b ->
-        is_derivable_wf C (l ∪ {[d]}) c ->
-        is_derivable_wf C (l ∪ {[ <{ b > d }> ]}) c
+        is_derivable_wf C (l +; d) c ->
+        is_derivable_wf C (l +; <{ b > d }>) c
     | wrl_impR C l b c :
-        is_derivable_wf C (l ∪ {[b]}) c ->
+        is_derivable_wf C (l +; b) c ->
         is_derivable_wf C l <{ b > c }>
     | wrl_forL C T l b c t :
         has_type C t T ->
-        is_derivable_wf C (l ∪ {[ subst_last C C t b ]}) c ->
-        is_derivable_wf C (l ∪ {[ <{for T, b}> ]}) c
+        is_derivable_wf C (l +; subst_last C C t b) c ->
+        is_derivable_wf C (l +; <{for T, b}>) c
     | wrl_forR C T l b sb :
         (forall t, t ∈ sb <-> in_supp b t) ->
         is_derivable_wf (C +: foldr ty_arr T (type_check_other <$> sb)) (sq_set_map (lift C) l) (
@@ -117,18 +125,113 @@ Module GLogic (SqSet : SQ_SET).
           sq_set_map (lift C) l ∪
           {[subst_last C (S C) (foldl tm_app (tm_lvl C) sb) b]}
         ) (lift C c) ->
-        is_derivable_wf C (l ∪ {[ <{ex T, b}> ]}) c
+        is_derivable_wf C (l +; <{ex T, b}>) c
     | wrl_exR C T l b t :
         has_type C t T ->
         is_derivable_wf C l (subst_last C C t b) ->
         is_derivable_wf C l <{ex T, b}>
     | wrl_nabL {T b} n (_ : ~ in_supp b (gtm_nom T n)) C l c :
-        is_derivable_wf C (l ∪ {[ subst_last C C (gtm_nom T n) b ]}) c ->
-        is_derivable_wf C (l ∪ {[ <{nab T, b}> ]}) c
+      is_derivable_wf C (l +; subst_last C C (gtm_nom T n) b) c ->
+      is_derivable_wf C (l +; <{nab T, b}>) c
     | wrl_nabR {T b} n (_ : ~ in_supp b (gtm_nom T n)) C l :
         is_derivable_wf C l (subst_last C C (gtm_nom T n) b) ->
         is_derivable_wf C l (<{nab T, b}>)
   .
+
+  Inductive is_derivable : context -> sq_set -> tm -> Prop :=
+    | rl_set C l m c :
+        l ≡ m ->
+        is_derivable C l c ->
+        is_derivable C m c
+    | rl_id (C : context) l a b :
+        tm_equiv C a b ->
+        is_derivable C (l +; a) b
+    | rl_cut C l m b c :
+        has_type C b ty_prp ->
+        is_derivable C l b ->
+        is_derivable C (m +; b) c ->
+        is_derivable C (l ∪ m) c
+    | rl_cL C l b c :
+        is_derivable C (l +; b +; b) c ->
+        is_derivable C (l +; b) c
+    | rl_botL C l c :
+        is_derivable C (l +; gtm_bot) c
+    | rl_topR C l :
+        is_derivable C l gtm_top
+    | rl_orL C l b c d :
+        is_derivable C (l +; b) c ->
+        is_derivable C (l +; d) c ->
+        is_derivable C (l +; <{ b \/ d }>) c
+    | rl_orR1 C l b c :
+        is_derivable C l b ->
+        is_derivable C l <{ b \/ c }>
+    | rl_orR2 C l b c :
+        is_derivable C l c ->
+        is_derivable C l <{ b \/ c }>
+    | rl_andL1 C l b c d :
+        is_derivable C (l +; b) c ->
+        is_derivable C (l +; <{ b /\ d }>) c
+    | rl_andL2 C l b c d :
+        is_derivable C (l +; d) c ->
+        is_derivable C (l +; <{ b /\ d }>) c
+    | rl_andR C l b c :
+        is_derivable C l b ->
+        is_derivable C l c ->
+        is_derivable C l <{ b /\ c }>
+    | rl_impL C l b c d :
+        is_derivable C l b ->
+        is_derivable C (l +; d) c ->
+        is_derivable C (l +; <{ b > d }>) c
+    | rl_impR C l b c :
+        is_derivable C (l +; b) c ->
+        is_derivable C l <{ b > c }>
+    | rl_forL C T l b c t :
+        has_type C t T ->
+        is_derivable C (l +; subst_last C C t b) c ->
+        is_derivable C (l +; <{for T, b}>) c
+    | rl_forR C T l b sb :
+        (forall t, t ∈ sb <-> in_supp b t) ->
+        is_derivable (C +: foldr ty_arr T (type_check_other <$> sb)) (sq_set_map (lift C) l) (
+          subst_last C (S C) (foldl tm_app (tm_lvl C) sb) b
+        ) ->
+        is_derivable C l <{for T, b}>
+    | rl_exL C T l b c sb :
+        (forall t, t ∈ sb <-> in_supp b t) ->
+        is_derivable (C +: foldr ty_arr T (type_check_other <$> sb)) (
+          sq_set_map (lift C) l ∪
+          {[subst_last C (S C) (foldl tm_app (tm_lvl C) sb) b]}
+        ) (lift C c) ->
+        is_derivable C (l +; <{ex T, b}>) c
+    | rl_exR C T l b t :
+        has_type C t T ->
+        is_derivable C l (subst_last C C t b) ->
+        is_derivable C l <{ex T, b}>
+    | rl_nabL {T b} n (_ : ~ in_supp b (gtm_nom T n)) C l c :
+    is_derivable C (l +; subst_last C C (gtm_nom T n) b) c ->
+    is_derivable C (l +; <{nab T, b}>) c
+    | rl_nabR {T b} n (_ : ~ in_supp b (gtm_nom T n)) C l :
+        is_derivable C l (subst_last C C (gtm_nom T n) b) ->
+        is_derivable C l (<{nab T, b}>)
+  .
+
+  Notation "[{ sig ; l --> B }]" := (is_derivable sig l B)
+    (sig custom stlc_ty, l custom stlc_tm, B custom stlc_tm) : stlc_scope.
+
+
+  Instance is_derivable_wf_Proper :
+    Proper ((=) ==> (≡) ==> (=) ==> iff) is_derivable_wf.
+  Proof.
+    intros ? ** ? ** ? **. subst.
+    split; intros H; eapply wrl_set; try apply H; easy.
+  Qed.
+
+  Instance is_derivable_Proper :
+    Proper ((=) ==> (≡) ==> (=) ==> iff) is_derivable.
+  Proof.
+    intros ? ** ? ** ? **. subst.
+    split; intros H; eapply rl_set; try apply H; easy.
+  Qed.
+
 
   Theorem has_type_fold C T h l t :
     Forall2 (fun x X => has_type C x X) l h ->
@@ -157,6 +260,24 @@ Module GLogic (SqSet : SQ_SET).
       + constructor. set_unfold. eapply in_supp_other. auto.
       + set_unfold. auto.
   Qed.
+
+  Theorem has_type_fold2_2 C T sb b :
+    (forall t, t ∈ sb -> in_supp b t) ->
+    has_type (C +: T) b ty_prp ->
+    has_type (C +: foldr ty_arr T (type_check_other <$> sb)) (subst_last C (S C) (foldl tm_app (tm_lvl C) sb) b) -[ o ]-.
+  Proof.
+    intros.
+    eapply has_type_subst_last1.
+    - tm_simpl. lia.
+    - intros. tm_simpl. now rewrite decide_True.
+    - eapply has_type_fold; tm_simpl; [|rewrite decide_False; intuition lia].
+      remember (C +: foldr ty_arr T (type_check_other <$> sb)) as D eqn : ED.
+      clear ED H0. induction sb; simpl in *; constructor.
+      + constructor. set_unfold. eapply in_supp_other. auto.
+      + set_unfold. auto.
+    - assumption.
+  Qed.
+
   Theorem is_derivable_wf_wf C l c : is_derivable_wf C l c -> wf_sequent C l c.
   Proof.
     intros D. unfold wf_sequent. induction D; simpl in *.
@@ -212,101 +333,44 @@ Module GLogic (SqSet : SQ_SET).
       now constructor.
   Qed.
 
-
-  Inductive is_derivable : context -> sq_set -> tm -> Prop :=
-    | rl_set C l m c :
-        l ≡ m ->
-        is_derivable C l c ->
-        is_derivable C m c
-    | rl_id (C : context) l a b :
-        tm_equiv C a b ->
-        is_derivable C (l ∪ {[a]}) b
-    | rl_cut C l m b c :
-        has_type C b ty_prp ->
-        is_derivable C l b ->
-        is_derivable C (m ∪ {[b]}) c ->
-        is_derivable C (l ∪ m) c
-    | rl_cL C l b c :
-        is_derivable C (l ∪ {[b; b]}) c ->
-        is_derivable C (l ∪ {[b]}) c
-    | rl_botL C l c :
-        is_derivable C (l ∪ {[gtm_bot]}) c
-    | rl_topR C l :
-        is_derivable C l gtm_top
-    | rl_orL C l b c d :
-        is_derivable C (l ∪ {[b]}) c ->
-        is_derivable C (l ∪ {[d]}) c ->
-        is_derivable C (l ∪ {[ <{ b \/ d }> ]}) c
-    | rl_orR1 C l b c :
-        is_derivable C l b ->
-        is_derivable C l <{ b \/ c }>
-    | rl_orR2 C l b c :
-        is_derivable C l c ->
-        is_derivable C l <{ b \/ c }>
-    | rl_andL1 C l b c d :
-        is_derivable C (l ∪ {[b]}) c ->
-        is_derivable C (l ∪ {[ <{ b /\ d }> ]}) c
-    | rl_andL2 C l b c d :
-        is_derivable C (l ∪ {[d]}) c ->
-        is_derivable C (l ∪ {[ <{ b /\ d }> ]}) c
-    | rl_andR C l b c :
-        is_derivable C l b ->
-        is_derivable C l c ->
-        is_derivable C l <{ b /\ c }>
-    | rl_impL C l b c d :
-        is_derivable C l b ->
-        is_derivable C (l ∪ {[d]}) c ->
-        is_derivable C (l ∪ {[ <{ b > d }> ]}) c
-    | rl_impR C l b c :
-        is_derivable C (l ∪ {[b]}) c ->
-        is_derivable C l <{ b > c }>
-    | rl_forL C T l b c t :
-        has_type C t T ->
-        is_derivable C (l ∪ {[ subst_last C C t b ]}) c ->
-        is_derivable C (l ∪ {[ <{for T, b}> ]}) c
-    | rl_forR C T l b sb :
-        (forall t, t ∈ sb <-> in_supp b t) ->
-        is_derivable (C +: foldr ty_arr T (type_check_other <$> sb)) (sq_set_map (lift C) l) (
-          subst_last C (S C) (foldl tm_app (tm_lvl C) sb) b
-        ) ->
-        is_derivable C l <{for T, b}>
-    | rl_exL C T l b c sb :
-        (forall t, t ∈ sb <-> in_supp b t) ->
-        is_derivable (C +: foldr ty_arr T (type_check_other <$> sb)) (
-          sq_set_map (lift C) l ∪
-          {[subst_last C (S C) (foldl tm_app (tm_lvl C) sb) b]}
-        ) (lift C c) ->
-        is_derivable C (l ∪ {[ <{ex T, b}> ]}) c
-    | rl_exR C T l b t :
-        has_type C t T ->
-        is_derivable C l (subst_last C C t b) ->
-        is_derivable C l <{ex T, b}>
-    | rl_nabL {T b} n (_ : ~ in_supp b (gtm_nom T n)) C l c :
-        is_derivable C (l ∪ {[ subst_last C C (gtm_nom T n) b ]}) c ->
-        is_derivable C (l ∪ {[ <{nab T, b}> ]}) c
-    | rl_nabR {T b} n (_ : ~ in_supp b (gtm_nom T n)) C l :
-        is_derivable C l (subst_last C C (gtm_nom T n) b) ->
-        is_derivable C l (<{nab T, b}>)
-  .
-
-  Notation "[{ sig ; l --> B }]" := (is_derivable sig l B)
-    (sig custom stlc_ty, l custom stlc_tm, B custom stlc_tm) : stlc_scope.
-
-  Notation "∅" := empty (in custom stlc_ty) : stlc_scope.
-  Notation "∅" := empty (in custom stlc_tm) : stlc_scope.
-  Notation "s +: x" := (s ∪ {[x]}) (in custom stlc_tm at level 50, left associativity) : stlc_scope.
-  Notation "∅" := empty : stdpp_scope.
-  Notation "{[ x ]}" := (singleton x) (in custom stlc_tm) : stlc_scope.
-
-  Theorem union_empty (X : sq_set) : ∅ ∪ X ≡ X.
-  Proof. set_unfold. intuition. Qed.
-
-  Instance is_derivable_Proper : Proper ((=) ==> (≡) ==> (=) ==> iff) is_derivable.
+  Theorem rl_wL C l m c :
+    [{ C; m --> c }] -> [{ C; l ∪ m --> c }].
   Proof.
-    intros ? ** ? ** ? **. subst.
-    split; intros H; eapply rl_set; try apply H; easy.
+    revert C l m c.
+    assert (MU : forall C h l, sq_set_map (lift C) <{ h ∪ l }> ≡ (sq_set_map (lift C) h) ∪ (sq_set_map (lift C) l) ). {
+      intros C h1 h2 x. set_unfold. repeat rewrite sq_set_map_spec.
+      set_unfold. split.
+      - intros [y [Hy ->]]. destruct Hy; intuition eauto.
+      - intros [[y [Hy ->]] | [y [Hy ->]]]; eauto.
+    }
+    intros * H. revert l.
+    induction H; intros h; try rewrite union_assoc in *.
+    - now rewrite <- H.
+    - now apply rl_id.
+    - eapply rl_cut; eauto.
+    - apply rl_cL. specialize IHis_derivable with h.
+      now repeat rewrite union_assoc in *.
+    - apply rl_botL.
+    - apply rl_topR.
+    - apply rl_orL; now rewrite <- union_assoc.
+    - now apply rl_orR1.
+    - now apply rl_orR2.
+    - apply rl_andL1; now rewrite <- union_assoc.
+    - apply rl_andL2; now rewrite <- union_assoc.
+    - now apply rl_andR.
+    - apply rl_impL; [easy|]. now rewrite <- union_assoc.
+    - apply rl_impR. now rewrite <- union_assoc.
+    - eapply rl_forL; [eassumption|].
+      now rewrite <- union_assoc.
+    - eapply rl_forR; try eassumption.
+      now rewrite MU.
+    - eapply rl_exL; try eassumption.
+      now rewrite MU, <- union_assoc.
+    - eapply rl_exR; eauto.
+    - eapply rl_nabL; try eassumption.
+      now rewrite <- union_assoc.
+    - eapply rl_nabR; eauto.
   Qed.
-
 
   Theorem is_derivable_wf_is_derivable C l c :
     is_derivable_wf C l c -> [{ C; l --> c }].
@@ -317,14 +381,157 @@ Module GLogic (SqSet : SQ_SET).
     - eapply rl_cut; try eassumption.
       apply is_derivable_wf_wf in DW1. destruct DW1. assumption.
     - now apply rl_cL.
-  Abort.
+    - now apply rl_wL.
+    - rewrite <- union_empty. apply rl_botL.
+    - apply rl_topR.
+    - now apply rl_orL.
+    - now apply rl_orR1.
+    - now apply rl_orR2.
+    - now apply rl_andL1.
+    - now apply rl_andL2.
+    - now apply rl_andR.
+    - now apply rl_impL.
+    - now apply rl_impR.
+    - eapply rl_forL; eassumption.
+    - eapply rl_forR; eassumption.
+    - eapply rl_exL; eassumption.
+    - eapply rl_exR; eassumption.
+    - eapply rl_nabL; eassumption.
+    - eapply rl_nabR; eassumption.
+  Qed.
 
   Theorem is_derivable_is_derivable_wf C l c :
     wf_sequent C l c ->  [{ C; l --> c }] -> is_derivable_wf C l c.
   Proof.
-    intros W D. induction D.
+    intros W D. unfold wf_sequent, wf_sq_set in W. induction D.
     - eapply wrl_set; [eassumption|].
-  Abort.
+      apply IHD. set_solver.
+    - destruct W. unfold wf_sq_set in *. set_unfold.
+      apply wrl_wL; try auto.
+      apply wrl_id; auto.
+    - eapply wrl_cut.
+      + apply IHD1. unfold wf_sequent, wf_sq_set in *.
+        set_solver.
+      + apply IHD2. unfold wf_sequent, wf_sq_set in *.
+        set_solver.
+    - apply wrl_cL. apply IHD.
+      unfold wf_sequent, wf_sq_set in *. set_solver.
+    - unfold wf_sequent, wf_sq_set in *.
+      apply wrl_wL; [|apply wrl_botL]; set_solver.
+    - unfold wf_sequent, wf_sq_set in *.
+      assert (l ≡ l ∪ ∅); [set_solver|].
+      rewrite H. apply wrl_wL; [|apply wrl_topR].
+      clear H. set_solver.
+    - apply wrl_orL.
+      + apply IHD1. intuition. set_unfold. destruct H3; intuition.
+        subst. eapply has_type_app_inv2_l.
+        * apply H. now right.
+        * now apply ht_other2.
+      + apply IHD2. set_unfold. intuition. subst.
+        eapply has_type_app_inv2_r.
+        * apply H. now right.
+        * now apply ht_other2.
+    - destruct W as [W1 W2]. apply wrl_orR1.
+      + eapply has_type_app_inv2_r; [apply W2|].
+        now apply ht_other2.
+      + apply IHD. intuition.
+        eapply has_type_app_inv2_l; [apply W2|].
+        now apply ht_other2.
+    - destruct W as [W1 W2]. apply wrl_orR2.
+      + eapply has_type_app_inv2_l; [apply W2|].
+        now apply ht_other2.
+      + apply IHD. intuition.
+        eapply has_type_app_inv2_r; [apply W2|].
+        now apply ht_other2.
+    - destruct W as [W1 W2]. set_unfold. apply wrl_andL1.
+      + eapply has_type_app_inv2_r.
+        * apply W1. now right.
+        * now apply ht_other2.
+      + apply IHD. intuition. subst.
+        eapply has_type_app_inv2_l.
+        * apply W1. now right.
+        * now apply ht_other2.
+    - destruct W as [W1 W2]. set_unfold. apply wrl_andL2.
+      + eapply has_type_app_inv2_l.
+        * apply W1. now right.
+        * now apply ht_other2.
+      + apply IHD. intuition. subst.
+        eapply has_type_app_inv2_r.
+        * apply W1. now right.
+        * now apply ht_other2.
+    - destruct W as [W1 W2]. apply wrl_andR.
+      + apply IHD1. intuition.
+        eapply has_type_app_inv2_l; [apply W2|].
+        now apply ht_other2.
+      + apply IHD2. intuition.
+        eapply has_type_app_inv2_r; [apply W2|].
+        now apply ht_other2.
+    - destruct W as [W1 W2]. set_unfold. apply wrl_impL.
+      + apply IHD1. intuition.
+        eapply has_type_app_inv2_l.
+        * apply W1. now right.
+        * now apply ht_other2.
+      + apply IHD2. intuition. subst.
+        eapply has_type_app_inv2_r.
+        * apply W1. now right.
+        * now apply ht_other2.
+    - destruct W as [W1 W2]. set_unfold. apply wrl_impR.
+      apply IHD. intuition.
+      + subst. eapply has_type_app_inv2_l; [apply W2|].
+        now apply ht_other2.
+      + eapply has_type_app_inv2_r; [apply W2|].
+        now apply ht_other2.
+    - destruct W as [W1 W2]. set_unfold. eapply wrl_forL; [eassumption|].
+      apply IHD. intuition. subst.
+      eapply has_type_subst_last_s1; [eassumption|].
+      eapply has_type_abs_inv.
+      eapply has_type_app_inv.
+      + apply W1. now right.
+      + now apply ht_other2.
+    - destruct W as [W1 W2]. set_unfold. eapply wrl_forR; [eassumption|].
+      apply IHD. intuition.
+      + apply sq_set_map_spec in H1 as [a [Ha1 Ha2]]. subst.
+        apply has_type_lift1. auto.
+      + apply has_type_fold2_2.
+        * apply H.
+        * eapply has_type_abs_inv.
+          eapply has_type_app_inv; [apply W2|].
+          now apply ht_other2.
+    - destruct W as [W1 W2]. set_unfold. eapply wrl_exL; [eassumption|].
+      apply IHD. intuition.
+      + apply sq_set_map_spec in H2 as [a [Ha1 Ha2]]. subst.
+        apply has_type_lift1. auto.
+      + subst. apply has_type_fold2_2.
+        * apply H.
+        * eapply has_type_abs_inv.
+          eapply has_type_app_inv.
+          -- apply W1. now right.
+          -- now apply ht_other2.
+      + now apply has_type_lift1.
+    - destruct W as [W1 W2]. set_unfold. eapply wrl_exR; [eassumption|].
+      apply IHD. intuition.
+      eapply has_type_subst_last_s1; [eassumption|].
+      eapply has_type_abs_inv.
+      eapply has_type_app_inv.
+      + apply W2.
+      + now apply ht_other2.
+    - destruct W as [W1 W2]. set_unfold. eapply wrl_nabL; [eassumption|].
+      apply IHD. intuition. subst.
+      eapply has_type_subst_last_s1.
+      + now apply ht_other.
+      + eapply has_type_abs_inv.
+        eapply has_type_app_inv.
+        * apply W1. now right.
+        * now apply ht_other2.
+    - destruct W as [W1 W2]. set_unfold. eapply wrl_nabR; [eassumption|].
+      apply IHD. intuition.
+      eapply has_type_subst_last_s1.
+      + now apply ht_other.
+      + eapply has_type_abs_inv.
+        eapply has_type_app_inv.
+        * apply W2.
+        * now apply ht_other2.
+  Qed.
 
 
   Theorem nom_in_supp b T : exists a, ~ in_supp b (gtm_nom T a).
@@ -345,11 +552,11 @@ Module GLogic (SqSet : SQ_SET).
   Ltac rl_nabL n := edestruct rl_nabL2 as [n ?X ?H]; apply H; clear H.
 
   Theorem sq_set_swap (l : sq_set) a b :
-    <{ l +: a +: b }> ≡ <{ l +: b +: a }>.
+    <{ l +; a +; b }> ≡ <{ l +; b +; a }>.
   Proof. set_unfold. intuition. Qed.
 
   Theorem contrapositive C l b c :
-    [{ C ; l +: b --> c }] -> [{ C ; l +: ~ c --> ~ b }].
+    [{ C ; l +; b --> c }] -> [{ C ; l +; ~ c --> ~ b }].
   Proof.
     intros H.
     apply rl_impR. rewrite sq_set_swap.
