theories/sets.v
@@ -1,0 +1,10 @@
+From stdpp Require Export sets.
+
+
+Theorem union_empty `{SemiSet T C} (X : C) : ∅ ∪ X ≡ X.
+Proof. set_solver. Qed.
+
+Theorem union_assoc `{SemiSet T C} (a b c : C) :
+  a ∪ (b ∪ c) ≡ a ∪ b ∪ c.
+Proof. set_solver. Qed.
+
